@prefix mv: <http://purl.org/net/mobivoc/> .
@prefix owl: <http://www.w3.org/2002/07/owl#> .
@prefix rdf: <http://www.w3.org/1999/02/22-rdf-syntax-ns#> .
@prefix rdfs: <http://www.w3.org/2000/01/rdf-schema#> .
@prefix skos: <http://www.w3.org/2004/02/skos/core#> .

# CLASSES

mv:BicycleDockingStation
  a rdfs:Class , owl:Class ;
  rdfs:comment "A docking station of a bicycle sharing system for picking up and returning bicycles." ;
  rdfs:label "bicycle docking station"@en , "Fahrradstation"@de .
  

 
#PROPERTIES

mv:dockingStationNumber
  a rdf:Property , owl:DatatypeProperty ;
  rdfs:label "docking station number"@en , "Stationsnummer"@de ;
  rdfs:comment "Identification number of the bicycle docking station." ;
  rdfs:domain mv:BicycleDockingStation ;
  rdfs:range rdfs:Literal .
  
mv:numberOfDockingPoints
  a rdf:Property , owl:DatatypeProperty ;
  rdfs:label "number of docking points"@en , "Anzahl Fahrradstellpl채tze"@de ;
  rdfs:comment "Indicates the number of docking points for bicycles." ;
  rdfs:domain mv:BicycleDockingStation ;
  rdfs:range rdfs:Literal .
  
mv:numberOfBicyclesAvailable
  a rdf:Property , owl:DatatypeProperty ;
  rdfs:label "number of bicycles available"@en , "Anzahl verf체gbarer Fahrr채der"@de ;
  rdfs:comment "Indicates the number of bicycles available at the docking station." ;
  rdfs:domain mv:BicycleDockingStation ;
  rdfs:range rdfs:Literal .
  
mv:numberOfSpacesAvailable
  a rdf:Property , owl:DatatypeProperty ;
  rdfs:label "number of spaces available"@en , "Anzahl freier Stellpl채tze"@de ;
  rdfs:comment "Indicates the number of spaces available at the docking station." ;
  rdfs:domain mv:BicycleDockingStation ;
  rdfs:range rdfs:Literal .
