@prefix mv: <http://eccenca.com/mobivoc/> .
@prefix owl: <http://www.w3.org/2002/07/owl#> .
@prefix rdf: <http://www.w3.org/1999/02/22-rdf-syntax-ns#> .
@prefix rdfs: <http://www.w3.org/2000/01/rdf-schema#> .
@prefix skos: <http://www.w3.org/2004/02/skos/core#> .

mv:Vehicle
	a rdfs:Class , owl:Class ;
	rdfs:comment "A vehicle is a mobile machine that transports people or cargo." ;
	rdfs:seeAlso <https://en.wikipedia.org/wiki/Vehicle> ;
	rdfs:label "vehicle"@en , "Auto"@de .
	
mv:FuelVehicle
	rdfs:subClassOf mv:Vehicle ;
	rdfs:comment "A vehicle which runs with fuel(gas)." ;
	rdfs:label "Fuel Vehicle"@en , "KraftstoffAuto"@de .
	
mv:BatteryElectricVehicle
	rdfs:subClassOf mv:Vehicle ;
	rdfs:comment "A type of electric vehicle that uses chemical energy stored in rechargeable battery packs." ;
	rdfs:seeAlso <https://en.wikipedia.org/wiki/Battery_electric_vehicle> ;
	rdfs:label "Battery Electric Vehicle"@en , "BatterieElektroAuto"@de .

mv:PlugInHybridElectricVehicle
	rdfs:subClassOf mv:Vehicle ;
	rdfs:comment "A type of hybrid and electric vehicle that combines a conventional internal combustion engine (ICE) propulsion system with an electric propulsion system" ;
	rdfs:seeAlso <https://en.wikipedia.org/wiki/Plug-in_hybrid> ;
	rdfs:label "PlugIn Hybrid Electric Vehicle"@en , "PlugInHybridElektroAuto"@de .


#Properties 

mv:hasHeight
	a rdf:Property , owl:DatatypeProperty ;
	rdfs:comment "Indicates the height of the vehicle." ;
	rdfs:label "Height"@en , "HÃ¶he"@de ;
	rdfs:domain mv:Vehicle ;
	rdfs:range mv:integer .
	
mv:usesFuel
	a rdf:Property , owl:DatatypeProperty ;
	rdfs:comment "Indicates if the specific vehicle uses fuel(gas)." ;
	rdfs:label "uses Fuel"@en , "benutzt Gas"@de ;
	rdfs:domain mv:Vehicle ;
	rdfs:range mv:boolean .
	
mv:usesBattery
	a rdf:Property , owl:DatatypeProperty ;
	rdfs:comment "Indicates if the specific vehicle uses battery." ;
	rdfs:label "uses Battery"@en , "benutzt Batterie"@de ;
	rdfs:domain mv:Vehicle ;
	rdfs:range mv:boolean .